refocusing/empty_search_order.v
@@ -1,0 +1,66 @@
+Require Import RelationClasses
+               Program
+               refocusing_semantics.
+
+Module Empty_search_order
+  (Import R : PRE_RED_SEM)
+  (Import RF: RED_STRATEGY_STEP_FUNCTIONS R).
+
+  Inductive elem_context_in k : Type := 
+  | ec_in : forall k' : ckind, elem_context_kinded k k' -> elem_context_in k.
+  Arguments ec_in {k} _ _.
+  Coercion ec_kinded_to_in {k1 k2} (ec : elem_context_kinded k1 k2) := ec_in k2 ec.
+
+  Definition search_order (k : ckind) (t : term) (ec ec0 : elem_context_in k) : Prop := False.
+
+  Notation "t |~  ec1 << ec2 "     := (search_order _ t ec1 ec2)
+                                   (at level 70, ec1, ec2 at level 50, no associativity).
+  Notation "k , t |~  ec1 << ec2 " := (search_order k t ec1 ec2)
+                                (at level 70, t, ec1, ec2 at level 50, no associativity).
+
+  Definition so_maximal {k} (ec : elem_context_in k) t :=
+       forall (ec' : elem_context_in k), ~ t |~ ec << ec'.
+  Definition so_minimal {k} (ec : elem_context_in k) t :=
+       forall (ec' : elem_context_in k), ~ t |~ ec' << ec.
+  Definition so_predecessor                                                           {k}
+      (ec0 : elem_context_in k) (ec1 : elem_context_in k) t :=
+
+      (*1*) t |~ ec0 << ec1 /\
+      (*2*)                                              forall (ec : elem_context_in k),
+            t |~ ec << ec1  ->  ~ t |~ ec0 << ec.
+  Hint Unfold so_maximal so_minimal so_predecessor.
+
+  Lemma dec_term_term_top : forall {k k'} t t' (ec : elem_context_kinded k k'),
+          dec_term t k = ed_dec _ t' ec -> so_maximal ec t.
+  Proof. intros ? ? ? ? ? ? ? []. Qed.
+
+  Lemma dec_context_red_bot :  forall {k k'} (v : value k') {r : redex k}
+                                                         (ec : elem_context_kinded k k'),
+          dec_context ec v = ed_red r -> so_minimal ec ec:[v].
+  Proof. intros ? ? ? ? ? ? ? []. Qed.
+
+  Lemma dec_context_val_bot : forall {k k'} (v : value k') {v' : value k}
+      (ec : elem_context_kinded k k'),
+      dec_context ec v = ed_val v' -> so_minimal ec ec:[v].
+  Proof. intros ? ? ? ? ? ? ? []. Qed.
+
+  Lemma elem_context_det :         forall {k0 k1 k2} t (ec0 : elem_context_kinded k0 k1)
+                                                       (ec1 : elem_context_kinded k0 k2),
+
+      t |~ ec0 << ec1 -> exists (v : value k2), t = ec1:[v].
+  Proof. intros ? ? ? t ec0 ec1 []. Qed.
+
+  Lemma wf_search : forall k t, well_founded (search_order k t).
+  Proof. intros ? ? ?. apply Acc_intro. intros _ []. Qed.
+
+  Lemma search_order_trans : forall k t, Transitive (search_order k t).
+  Proof. intros ? ? ? ? ? []. Qed.
+
+  Lemma search_order_comp_fi :
+      forall t k k' k'' (ec0 : elem_context_kinded k k')
+                        (ec1 : elem_context_kinded k k''),
+          k, t |~ ec0 << ec1 ->
+              immediate_ec ec0 t /\ immediate_ec ec1 t.
+  Proof. intros ? ? ? ? ? ? []. Qed.
+
+End Empty_search_order.
